Add some proof support to Candidate definitions
- Add FMapUnfold typeclass
- Add lots of list reasoning automation including for NoDup
- Make mbind Typeclasses Opaque (and fix Exec.v)
- Prove specification for event_list event_map and collect_all in
  Candidate

Common/CList.v
@@ -1,7 +1,16 @@
-Require Import CBase CBool.
+Require Import CBase CBool CMaps.
 From stdpp Require Import base.
 From stdpp Require Export list.
 From stdpp Require Export listset.
+
+Global Instance proper_list_mbind A B :
+  Proper (pointwise_relation A (=) ==> (=@{list A}) ==> (=@{list B})) mbind.
+Proof.
+  intros x y H ? l ->.
+  unfold pointwise_relation in H.
+  induction l; hauto q:on.
+Qed.
+
 
 (*** List simplification ***)
 
@@ -166,7 +175,58 @@ Lemma is_emptyb_eq_nil {A} (l : list A) : is_true (is_emptyb l) <-> l = [].
 Proof. sauto lq:on. Qed.
 #[global] Hint Rewrite @is_emptyb_eq_nil: brefl.
 
-Definition enumerate {A} (l : list A) : list (nat * A) := zip_with pair (seq 0 (length l)) l.
+Definition enumerate {A} (l : list A) : list (nat * A) :=
+  zip_with pair (seq 0 (length l)) l.
+#[global] Typeclasses Opaque enumerate.
+#[global] Typeclasses Opaque zip_with.
+
+
+Global Instance set_elem_of_zip_with A B C (x : C) (f : A → B → C) l1 l2:
+  SetUnfoldElemOf x (zip_with f l1 l2)
+    (∃ (n : nat) y z, l1 !! n = Some y ∧ l2 !! n = Some z ∧ f y z = x) | 10.
+Proof. tcclean. rewrite elem_of_lookup_zip_with. naive_solver. Qed.
+
+Global Instance set_elem_of_zip A B (x : A * B) l1 l2:
+  SetUnfoldElemOf x (zip l1 l2)
+    (∃ (n : nat), l1 !! n = Some x.1 ∧ l2 !! n = Some x.2).
+Proof. tcclean. set_unfold. hauto lq:on. Qed.
+
+Global Instance lookup_seq n i l:
+  LookupUnfold n (seq i l) (if decide (n < l) then Some (n + i) else None)%nat.
+Proof.
+  tcclean.
+  generalize dependent i.
+  generalize dependent n.
+  induction l; intros n i.
+  - compute_done.
+  - destruct n; cbn; try reflexivity.
+    rewrite IHl.
+    hauto l:on.
+Qed.
+
+Lemma lookup_seq_success (n i l m : nat):
+  (seq i l) !! n = Some m → m = (n + i)%nat.
+Proof. rewrite lookup_unfold. case_decide; naive_solver. Qed.
+
+Lemma lookup_length A (l : list A) n x :
+  l !! n = Some x → (n < length l)%nat.
+Proof. rewrite <- lookup_lt_is_Some. naive_solver. Qed.
+
+Ltac list_saturate :=
+  match goal with
+  | H : _ !! _ = Some _ |- _ => learn_hyp (lookup_length _ _ _ _ H)
+  | H : _ !! _ = Some _ |- _ => learn_hyp (elem_of_list_lookup_2 _ _ _ H)
+  end.
+
+Global Instance set_elem_of_enumerate A (x : nat * A) l:
+  SetUnfoldElemOf x (enumerate l) (l !! x.1 = Some x.2).
+Proof.
+  tcclean.
+  unfold enumerate.
+  set_unfold.
+  setoid_rewrite lookup_unfold.
+  hauto l:on simp+:eexists simp+:list_saturate.
+Qed.
 
 Section FilterMap.
   Context {A B : Type}.
@@ -191,3 +251,85 @@ End FilterMap.
 Lemma length_one_iff_singleton A (l : list A) :
   length l = 1 <-> exists a, l = [a].
 Proof. sauto lq: on rew:off. Qed.
+
+
+(*** Fmap Unfold ***)
+Class FMapUnfold {M : Type → Type} {fm : FMap M}
+  {A B} (f : A → B) (ma : M A) (mb : M B) := {fmap_unfold : f <$> ma = mb }.
+Global Hint Mode FMapUnfold + + + + + + - : typeclass_instances.
+
+Global Instance fmap_unfold_default `{FMap M} {A B} (f : A → B) (l : M A):
+  FMapUnfold f l (f <$> l) | 1000.
+Proof. tcclean. reflexivity. Qed.
+
+Global Instance fmap_unfold_list_app {A B} (f : A → B) l l' l2 l2':
+  FMapUnfold f l l2 → FMapUnfold f l' l2' →
+  FMapUnfold f (app l l') (app l2 l2').
+Proof. tcclean. apply fmap_app. Qed.
+
+Lemma list_bind_fmap A B C (l : list A) (f : A → list B) (g : B -> C):
+  g <$> (x ← l; f x) = x ← l; g <$> (f x).
+Proof.
+  induction l. { done. }
+  cbn.
+  rewrite fmap_unfold.
+  rewrite <- IHl.
+  reflexivity.
+Qed.
+Global Instance fmap_unfold_list_mbind {A B C} (f : B → C) (g : A → list B)  l l2:
+  (∀ x, FMapUnfold f (g x) (l2 x)) →
+  FMapUnfold f (x ← l; g x) (x ← l; l2 x).
+Proof. tcclean. apply list_bind_fmap. Qed.
+
+Global Instance fmap_unfold_let_pair {A B C D} (f : C → D) x
+  (l : A → B → list C) l2:
+  (∀ a b, FMapUnfold f (l a b) (l2 a b)) →
+  FMapUnfold f (let '(a, b) := x in l a b) (let '(a, b) := x in l2 a b).
+Proof. tcclean. destruct x. done. Qed.
+
+
+(*** NoDup management ***)
+
+Global Hint Resolve NoDup_nil_2 : nodup.
+Global Hint Resolve NoDup_cons_2 : nodup.
+Global Hint Rewrite @list.NoDup_cons : nodup.
+Global Hint Resolve NoDup_singleton : nodup.
+
+
+Lemma NoDup_zip_with_l {A B C} (f : A → B → C) l l':
+  (∀ x y x' y', f x x' = f y y' → x = y) → NoDup l →
+  NoDup (zip_with f l l').
+Proof.
+  intros Hinj HND.
+  generalize dependent l'.
+  induction l;
+    destruct l';
+    hauto l:on db:nodup simp+:list_saturate simp+:set_unfold.
+Qed.
+
+Lemma NoDup_zip_with_r {A B C} (f : A → B → C) l l':
+  (∀ x y x' y', f x x' = f y y' → x' = y') → NoDup l' →
+  NoDup (zip_with f l l').
+Proof.
+  intros Hinj HND.
+  generalize dependent l.
+  induction l';
+    destruct l;
+    hauto l:on db:nodup simp+:list_saturate simp+:set_unfold.
+Qed.
+
+Lemma NoDup_zip_l {A B} (l : list A) (l' : list B):
+  NoDup l → NoDup (zip l l').
+Proof. intro. apply NoDup_zip_with_l; naive_solver. Qed.
+
+Lemma NoDup_zip_r {A B} (l : list A) (l' : list B):
+  NoDup l' → NoDup (zip l l').
+Proof. intro. apply NoDup_zip_with_r; naive_solver. Qed.
+
+Lemma NoDup_enumerate A (l : list A) : NoDup (enumerate l).
+Proof.
+  unfold enumerate.
+  apply NoDup_zip_l.
+  apply NoDup_seq.
+Qed.
+Global Hint Resolve NoDup_enumerate : nodup.
